Spqr.lean
@@ -8,7 +8,11 @@ import Spqr.Specs.Encoding.Gf.GF16.AddAssign
 import Spqr.Specs.Encoding.Gf.GF16.ConstDiv
 import Spqr.Specs.Encoding.Gf.GF16.ConstMul
 import Spqr.Specs.Encoding.Gf.GF16.ConstSub
+import Spqr.Specs.Encoding.Gf.GF16.Div
+import Spqr.Specs.Encoding.Gf.GF16.DivImpl
 import Spqr.Specs.Encoding.Gf.GF16.Eq
+import Spqr.Specs.Encoding.Gf.GF16.Mul
+import Spqr.Specs.Encoding.Gf.GF16.MulAssign
 import Spqr.Specs.Encoding.Gf.GF16.New
 import Spqr.Specs.Encoding.Gf.GF16.ONE
 import Spqr.Specs.Encoding.Gf.GF16.Sub
